src/machine_inter_tests.v
@@ -1,0 +1,81 @@
+Require Import DTDT.syntax.
+Require Import DTDT.machine_inter.
+
+(* Example evaluations for the machine semantics. *)
+
+Definition machine_ref_ctx (Γ : ctx) : ctx :=
+  Γ ,,s "l" ↦ (TBase BNat, ENat 2).
+
+Definition machine_ref_update_fun : i_expr :=
+  EFix "f" "r" (TRef (TBase BNat)) (TBase BUnit)
+    (EIf (EEq (EGet (EVar "r")) (ENat 2))
+         (ESet (EVar "r") (ENat 7))
+         EFail).
+
+(* Example evaluation of a conditional that reads a reference and updates the store. *)
+Lemma eval_if_get_set_test : forall Γ,
+  (machine_ref_ctx Γ,
+   EIf (EEq (EGet (EVar "l")) (ENat 2))
+       (ESet (EVar "l") (ENat 5))
+       EFail) ↠*
+  (((Γ ,,s "l" ↦ (TBase BNat, ENat 2)) ,,s "l" ↦ (TBase BNat, ENat 5)), EUnit tt).
+Proof.
+  intros Γ.
+  unfold machine_ref_ctx.
+  eapply steps_step.
+  - eapply StepCtx with (E := ECIf ECHole (ESet (EVar "l") (ENat 5)) EFail).
+    eapply StepCtx with (E := ECEqL ECHole (ENat 2)).
+    eapply StepGet with (τ := TBase BNat) (v := ENat 2).
+    unfold store_ctx_lookup, ctx_add_store. cbn.
+    apply lookup_insert.
+  - eapply steps_step.
+    + eapply StepCtx with (E := ECIf ECHole (ESet (EVar "l") (ENat 5)) EFail).
+      apply StepEq.
+      * apply VNat.
+      * apply VNat.
+      * reflexivity.
+    + eapply steps_step.
+      * apply StepIfTrue.
+      * eapply steps_step.
+        -- eapply StepSet with (τ := TBase BNat) (e := ENat 2).
+           ++ apply VNat.
+           ++ unfold store_ctx_lookup, ctx_add_store. cbn.
+              apply lookup_insert.
+        -- apply steps_refl.
+Qed.
+
+(* Example evaluation of an application whose body performs a stateful reference update. *)
+Lemma eval_app_with_store_effect_test : forall Γ,
+  (machine_ref_ctx Γ,
+   EApp machine_ref_update_fun (EVar "l")) ↠*
+  (((Γ ,,s "l" ↦ (TBase BNat, ENat 2)) ,,s "l" ↦ (TBase BNat, ENat 7)), EUnit tt).
+Proof.
+  intros Γ.
+  unfold machine_ref_ctx, machine_ref_update_fun.
+  eapply steps_step.
+  - apply StepFix.
+    apply VLoc with (τ := TBase BNat) (v := ENat 2).
+    unfold store_ctx_lookup, ctx_add_store. cbn.
+    apply lookup_insert.
+  - simpl.
+    eapply steps_step.
+    + eapply StepCtx with (E := ECIf ECHole (ESet (EVar "l") (ENat 7)) EFail).
+      eapply StepCtx with (E := ECEqL ECHole (ENat 2)).
+      eapply StepGet with (τ := TBase BNat) (v := ENat 2).
+      unfold store_ctx_lookup, ctx_add_store. cbn.
+      apply lookup_insert.
+    + eapply steps_step.
+      * eapply StepCtx with (E := ECIf ECHole (ESet (EVar "l") (ENat 7)) EFail).
+        apply StepEq.
+        -- apply VNat.
+        -- apply VNat.
+        -- reflexivity.
+      * eapply steps_step.
+        -- apply StepIfTrue.
+        -- eapply steps_step.
+           ++ eapply StepSet with (τ := TBase BNat) (e := ENat 2).
+              ** apply VNat.
+              ** unfold store_ctx_lookup, ctx_add_store. cbn.
+                 apply lookup_insert.
+           ++ apply steps_refl.
+Qed.
