src/semantic_rules_inter_tests.v
@@ -1,0 +1,183 @@
+Require Import DTDT.syntax.
+Require Import DTDT.machine_inter.
+Require Import DTDT.entails_inter.
+Require Import DTDT.semantic_rules_inter.
+
+(* Example derivations for the internal judgments. *)
+
+(* Local tactics and lookup lemmas used by the semantic examples. *)
+Ltac solve_var :=
+  eapply StepVar;
+  unfold ctx_add_var, var_ctx_lookup;
+  simpl;
+  apply lookup_insert; simpl.
+
+Lemma var_lookup_add (Γ : ctx) x (τ : i_ty) e :
+  (Γ ,,v x ↦ (τ, e)) !!₁ x = Some (τ, e).
+Proof.
+  unfold var_ctx_lookup, ctx_add_var. cbn.
+  apply lookup_insert.
+Qed.
+
+Lemma var_lookup_add_ne (Γ : ctx) y (τ : i_ty) ey x (τ₂ : i_ty) e :
+  x <> y ->
+  var_ctx_lookup Γ x = Some (τ₂, e) ->
+  var_ctx_lookup (ctx_add_var Γ y τ ey) x = Some (τ₂, e).
+Proof.
+  intros Hneq Hlookup.
+  destruct Γ as [[vars consts] store].
+  unfold var_ctx_lookup, ctx_add_var in *. simpl in *.
+  assert (Hyx : y <> x) by congruence.
+  rewrite (lookup_insert_ne vars y x (τ, ey) Hyx).
+  exact Hlookup.
+Qed.
+
+Definition pure_nat_ctx : ctx :=
+  empty_ctx ,,v "n" ↦ (TBase BNat, ENat 2).
+
+Definition ref_nat_ctx : ctx :=
+  empty_ctx ,,s "l" ↦ (TBase BNat, ENat 2).
+
+Definition ref_inspecting_fun : i_expr :=
+  EFix "f" "r" (TRef (TBase BNat)) (TBase BNat)
+    (EIf (EEq (ENat 0) (ENat 0))
+         (EPlus (EGet (EVar "r")) (ENat 1))
+         (ENat 0)).
+
+(* Example pure typing derivation for a nested boolean/arithmetic formula. *)
+Lemma pure_guarded_arithmetic_test :
+  pure_nat_ctx ⊢pure
+    EImp (EEq (EVar "n") (ENat 2))
+         (EEq (EPlus (EVar "n") (ENat 1)) (ENat 3))
+    : TBase BBool.
+Proof.
+  apply PImp.
+  - eapply PEq.
+    + apply PVar with (τb := TBase BNat) (e := ENat 2).
+      * unfold pure_nat_ctx. apply var_lookup_add.
+      * reflexivity.
+    + apply PNat.
+  - eapply PEq.
+    + apply PPlus.
+      * apply PVar with (τb := TBase BNat) (e := ENat 2).
+        -- unfold pure_nat_ctx. apply var_lookup_add.
+        -- reflexivity.
+      * apply PNat.
+    + apply PNat.
+Qed.
+
+(* Example semantic subtyping derivation driven by a nontrivial implication witness. *)
+Lemma subtype_refinement_implication_test : forall Γ,
+  subtype Γ
+    (TSet "x" BNat (EEq (EVar "x") (ENat 3)))
+    (TSet "x" BNat (EOr (EEq (EVar "x") (ENat 3))
+                         (EEq (EVar "x") (ENat 4)))).
+Proof.
+  intro Γ.
+  eapply SSet with (c := 3).
+  - apply VSet with (v := ENat 3).
+    eapply PEq.
+    + apply PVar with (τb := TBase BNat) (e := ENat 3).
+      * apply var_lookup_add.
+      * reflexivity.
+    + apply PNat.
+  - apply VSet with (v := ENat 3).
+    apply POr.
+    + eapply PEq.
+      * apply PVar with (τb := TBase BNat) (e := ENat 3).
+        -- apply var_lookup_add.
+        -- reflexivity.
+      * apply PNat.
+    + eapply PEq.
+      * apply PVar with (τb := TBase BNat) (e := ENat 3).
+        -- apply var_lookup_add.
+        -- reflexivity.
+      * apply PNat.
+  - simpl.
+    eapply steps_step.
+    + eapply StepCtx with (E := ECImpL ECHole (EOr (EEq (EVar "x") (ENat 3)) (EEq (EVar "x") (ENat 4)))).
+      eapply StepCtx with (E := ECEqL ECHole (ENat 3)).
+      solve_var.
+    + eapply steps_step.
+      * eapply StepCtx with (E := ECImpL ECHole (EOr (EEq (EVar "x") (ENat 3)) (EEq (EVar "x") (ENat 4)))).
+        apply StepEq.
+        -- apply VNat.
+        -- apply VNat.
+        -- reflexivity.
+      * eapply steps_step.
+        -- eapply StepCtx with (E := ECImpR (EBool true) ECHole).
+           eapply StepCtx with (E := ECOrL ECHole (EEq (EVar "x") (ENat 4))).
+           eapply StepCtx with (E := ECEqL ECHole (ENat 3)).
+           solve_var.
+        -- eapply steps_step.
+           ++ eapply StepCtx with (E := ECImpR (EBool true) ECHole).
+              eapply StepCtx with (E := ECOrL ECHole (EEq (EVar "x") (ENat 4))).
+              apply StepEq.
+              ** apply VNat.
+              ** apply VNat.
+              ** reflexivity.
+           ++ eapply steps_step.
+              ** eapply StepCtx with (E := ECImpR (EBool true) ECHole).
+                 eapply StepCtx with (E := ECOrR (EBool true) ECHole).
+                 eapply StepCtx with (E := ECEqL ECHole (ENat 4)).
+                 solve_var.
+              ** eapply steps_step.
+                 --- eapply StepCtx with (E := ECImpR (EBool true) ECHole).
+                     eapply StepCtx with (E := ECOrR (EBool true) ECHole).
+                     apply StepEq.
+                     +++ apply VNat.
+                     +++ apply VNat.
+                     +++ reflexivity.
+                 --- eapply steps_step.
+                     +++ eapply StepCtx with (E := ECImpR (EBool true) ECHole).
+                         apply StepOr.
+                     +++ eapply steps_step.
+                         *** apply StepImp.
+                         *** apply steps_refl.
+Qed.
+
+(* Example typing derivation for a conditional that reads from the store. *)
+Lemma has_type_reference_conditional_test :
+  has_type ref_nat_ctx
+    (EIf (EEq (ENat 0) (ENat 0))
+         (EPlus (EGet (EVar "l")) (ENat 1))
+         (ENat 0))
+    (TBase BNat).
+Proof.
+  unfold ref_nat_ctx.
+  eapply TIf with (u := "u").
+  - eapply PEq; apply PNat.
+  - apply TPlus.
+    + eapply TGet.
+      apply TLoc with (v := ENat 2).
+      unfold store_ctx_lookup, ctx_add_var, ctx_add_store. cbn.
+      apply lookup_insert.
+    + apply TNat.
+  - apply TNat.
+Qed.
+
+(* Example typing derivation for a function that inspects a reference argument. *)
+Lemma has_type_reference_inspecting_function_test :
+  has_type empty_ctx ref_inspecting_fun
+    (TArrDep "r" (TRef (TBase BNat)) (TBase BNat)).
+Proof.
+  unfold ref_inspecting_fun.
+  eapply TFun with (exp :=
+    EFix "f" "r" (TRef (TBase BNat)) (TBase BNat)
+      (EIf (EEq (ENat 0) (ENat 0))
+           (EPlus (EGet (EVar "r")) (ENat 1))
+           (ENat 0))).
+  - apply VFunDep with (v := EVar "r").
+    + apply VRef. apply VBase.
+    + apply VBase.
+  - eapply TIf with (u := "u").
+    + eapply PEq; apply PNat.
+    + apply TPlus.
+      * eapply TGet.
+        eapply TVar with (v := "r") (e := EVar "r").
+        eapply var_lookup_add_ne.
+        -- discriminate.
+        -- apply var_lookup_add.
+      * apply TNat.
+    + apply TNat.
+Qed.
