src/type_directed_translation_tests.v
@@ -1,0 +1,182 @@
+Require Import DTDT.syntax.
+Require Import DTDT.machine_inter.
+Require Import DTDT.semantic_rules_inter.
+Require Import DTDT.semantic_rules_surf.
+Require Import DTDT.type_directed_translation.
+
+(* Example derivations for translation, coercion, and translated typing. *)
+
+Definition surf_newref_nat_expr : expr :=
+  ExNewRef (TyBase BNat) (ExNat 5).
+
+Definition inter_newref_nat_expr : i_expr :=
+  ENewRef (TBase BNat) (ENat 5).
+
+Definition inter_dref_nat_expr : i_expr :=
+  EPair
+    (EFix "" "u" (TBase BUnit) (TBase BNat) (EGet inter_newref_nat_expr))
+    (EFix "" "x" (TBase BNat) (TBase BUnit) (ESet inter_newref_nat_expr (EVar "x"))).
+
+Definition surf_dref_if_nat_expr : expr :=
+  ExIf (ExBool true)
+       (ExGetDep (ExDeRef surf_newref_nat_expr))
+       (ExNat 0).
+
+Definition inter_dref_if_nat_expr : i_expr :=
+  EIf (EBool true) (dget inter_dref_nat_expr) (ENat 0).
+
+Definition surf_dref_set_if_unit_expr : expr :=
+  ExIf (ExBool true)
+       (ExSetDep (ExDeRef surf_newref_nat_expr) (ExNat 7))
+       (ExUnit tt).
+
+Definition inter_dref_set_if_unit_expr : i_expr :=
+  EIf (EBool true) (dset inter_dref_nat_expr (ENat 7)) (EUnit tt).
+
+Definition surf_const_dep_fun_nat_expr : expr :=
+  ExFix "f" "x" (TyBase BNat) (TyBase BNat) (ExNat 0).
+
+Definition surf_impure_app_ctx : ctx_surf :=
+  ((empty_ctx_surf ,,sv "f" ↦
+      ((TyArrDep "x" (TyBase BNat) (TyBase BNat)), surf_const_dep_fun_nat_expr))
+    ,,sv "r" ↦ (TyRef (TyBase BNat), ExVar "r")).
+
+Definition erased_dep_fun_var_term : i_expr :=
+  expr_subst "y" (EVar "f")
+    (EFix (fresh_string_list (exp_vars (EApp (EVar "y") (EVar "x"))))
+      "x" (TBase BNat) (TBase BNat) (EApp (EVar "y") (EVar "x"))).
+
+(* Example coercion from an ordinary reference to an encoded dynamic reference. *)
+Lemma coerce_newref_nat_to_dref_example : forall Γ,
+  coerce sim Γ
+    inter_newref_nat_expr (TRef (TBase BNat))
+    inter_dref_nat_expr (dref_encoding (TBase BNat)).
+Proof.
+  intro Γ.
+  unfold inter_dref_nat_expr, inter_newref_nat_expr.
+  eapply CRefToDRef with
+    (y := "y")
+    (u := "u")
+    (x := "x")
+    (get_body := EGet (EVar "y"))
+    (set_arg := EVar "x")
+    (vy := EUnit tt)
+    (vx := ENat 0).
+  - reflexivity.
+  - reflexivity.
+  - reflexivity.
+  - apply CSub. apply SBase.
+  - apply CSub. apply SBase.
+Qed.
+
+(* Example translation of dynamic-reference introduction. *)
+Lemma has_type_surf_deref_nat_example : forall Γ,
+  has_type_surf sim Γ
+    (ExDeRef surf_newref_nat_expr)
+    inter_dref_nat_expr
+    (dref_encoding (TBase BNat)).
+Proof.
+  intro Γ.
+  eapply (@ATDeRef sim _ surf_newref_nat_expr inter_newref_nat_expr inter_dref_nat_expr (TyBase BNat)).
+  - reflexivity.
+  - reflexivity.
+  - unfold surf_newref_nat_expr, inter_newref_nat_expr.
+    eapply ATNewRef with (e' := ENat 5) (e'' := ENat 5).
+    + apply VRefS. apply VBaseS.
+    + apply ATNat.
+    + apply CSub. apply SBase.
+  - apply coerce_newref_nat_to_dref_example.
+Qed.
+
+(* Example translation derivation for a conditional that reads through a dynamic reference. *)
+Lemma has_type_surf_dref_if_nat_test :
+  has_type_surf sim empty_ctx_surf
+    surf_dref_if_nat_expr
+    inter_dref_if_nat_expr
+    (TBase BNat).
+Proof.
+  unfold surf_dref_if_nat_expr, inter_dref_if_nat_expr.
+  simple eapply (@ATIfPure sim empty_ctx_surf
+    (ExBool true)
+    (ExGetDep (ExDeRef surf_newref_nat_expr))
+    (ExNat 0)
+    (dget inter_dref_nat_expr) (dget inter_dref_nat_expr)
+    (ENat 0) (ENat 0)
+    (TBase BNat) (TBase BNat) (TBase BNat) "u").
+  - apply PBoolS.
+  - eapply ATGetDep with (e' := inter_dref_nat_expr) (τ := TyBase BNat).
+    apply has_type_surf_deref_nat_example.
+  - apply ATNat.
+  - apply CSub. apply SBase.
+  - apply CSub. apply SBase.
+  - apply JoinBase.
+Qed.
+
+(* Example translation derivation for a conditional that writes through a dynamic reference. *)
+Lemma has_type_surf_dref_set_if_unit_test :
+  has_type_surf sim empty_ctx_surf
+    surf_dref_set_if_unit_expr
+    inter_dref_set_if_unit_expr
+    (TBase BUnit).
+Proof.
+  unfold surf_dref_set_if_unit_expr, inter_dref_set_if_unit_expr.
+  simple eapply (@ATIfPure sim empty_ctx_surf
+    (ExBool true)
+    (ExSetDep (ExDeRef surf_newref_nat_expr) (ExNat 7))
+    (ExUnit tt)
+    (dset inter_dref_nat_expr (ENat 7)) (dset inter_dref_nat_expr (ENat 7))
+    (EUnit tt) (EUnit tt)
+    (TBase BUnit) (TBase BUnit) (TBase BUnit) "u").
+  - apply PBoolS.
+  - eapply ATSetDep with
+      (e1' := inter_dref_nat_expr)
+      (e2' := ENat 7)
+      (e2'' := ENat 7)
+      (τ := TyBase BNat)
+      (τ' := TBase BNat).
+    + apply has_type_surf_deref_nat_example.
+    + apply ATNat.
+    + apply CSub. apply SBase.
+  - apply ATUnit.
+  - apply CSub. apply SBase.
+  - apply CSub. apply SBase.
+  - apply JoinBase.
+Qed.
+
+(* Example translation derivation for impure application through function erasure. *)
+Lemma has_type_surf_app_impure_nat_test :
+  has_type_surf sim surf_impure_app_ctx
+    (ExApp (ExVar "f") (ExGet (ExVar "r")))
+    (EApp erased_dep_fun_var_term (EGet (EVar "r")))
+    (TBase BNat).
+Proof.
+  simple eapply (@ATAppImPure sim surf_impure_app_ctx
+    (ExVar "f") (ExGet (ExVar "r"))
+    (EVar "f") erased_dep_fun_var_term
+    (EGet (EVar "r")) (EGet (EVar "r"))
+    "x" (TBase BNat) (TBase BNat) (TBase BNat)).
+  - simple eapply (@ATVar sim surf_impure_app_ctx "f"
+      (TyArrDep "x" (TyBase BNat) (TyBase BNat)) surf_const_dep_fun_nat_expr).
+    + unfold surf_impure_app_ctx, var_ctx_lookup_surf, ctx_add_var_surf. compute. reflexivity.
+    + intro H.
+      inversion H; subst.
+      destruct τb; simpl in *; try contradiction; discriminate.
+  - simple eapply (@ATGet sim surf_impure_app_ctx (ExVar "r") (EVar "r") (TBase BNat)).
+    simple eapply (@ATVar sim surf_impure_app_ctx "r" (TyRef (TyBase BNat)) (ExVar "r")).
+    + unfold surf_impure_app_ctx, var_ctx_lookup_surf, ctx_add_var_surf. compute. reflexivity.
+    + intro H.
+      inversion H; subst.
+      destruct τb; simpl in *; try contradiction; discriminate.
+  - apply CSub. apply SBase.
+  - intro Hpure.
+    specialize (Hpure (TBase BNat)).
+    inversion Hpure.
+  - unfold erased_dep_fun_var_term.
+    eapply CFunEraseDep with
+      (y := "y")
+      (body := EApp (EVar "y") (EVar "x"))
+      (vy := ENat 0)
+      (vx := ENat 0).
+    + reflexivity.
+    + apply CSub. apply SBase.
+Qed.
